\section{Формулы}

\begin{equation}\label{eq:formul}
	l_1\cdot\cos(\phi)+l_2\cdot\cos\left(\arcsin\left(\dfrac{e_1-l_1\cdot\sin(\phi)}{l_2}\right)\right)=x(\phi)
\end{equation}

\begin{figure}[H]
	\centering
	\begin{tikzpicture}
		\begin{axis}[
			grid = major,
			axis equal image = false,
			width=16.5cm,
			]
			\addplot plot table {graphs/1.dat};
		\end{axis}
	\end{tikzpicture}
\end{figure}
\newpage
\begin{equation}\label{eq:xc1}
	l_1\cdot\cos(\phi_n)+l_2\cdot\cos\left(\arcsin\left(\dfrac{e_1-l_1\cdot\sin(\phi_n)}{l_2}\right)\right)=x_{c_1}
\end{equation}

\begin{multline}\label{eq:xc1calc}
	0.02\cdot\cos(\pi)+0.035\cdot\cos\left(\arcsin\left(\dfrac{0.25\cdot 0.02-0.02\cdot\sin(\pi)}{0.035}\right)\right)=\\
	=-0.02+0.035\cdot0.0285714=0.014641=x_{c_1}
\end{multline}

\begin{equation}\label{eq:yc1}
	y_{c_1} = 0
\end{equation}

\begin{equation}\label{eq:xc2}
	l_1\cdot\cos(\phi_k)+l_2\cdot\cos\left(\arcsin\left(\dfrac{e_1-l_1\cdot\sin(\phi_k)}{l_2}\right)\right)=x_{c_2}
\end{equation}

\begin{equation}\label{eq:yc2}
	y_{c_2}=0
\end{equation}
\newpage
Координаты $ A $:

\begin{equation}\label{eq:xA}
	x_A=l_1\cdot\cos(\phi)
\end{equation}

\begin{figure}[H]
	\centering
	\begin{tikzpicture}
		\begin{axis}[
			grid = major,
			axis equal image = false,
			width=16.5cm,
			]
			\addplot plot table {graphs/6.dat};
		\end{axis}
	\end{tikzpicture}
\end{figure}
\newpage
\begin{equation}\label{eq:yA}
	y_A=l_1\cdot\sin(\phi)
\end{equation}

\begin{figure}[H]
	\centering
	\begin{tikzpicture}
		\begin{axis}[
			grid = major,
			axis equal image = false,
			width=16.5cm,
			]
			\addplot plot table {graphs/7.dat};
		\end{axis}
	\end{tikzpicture}
\end{figure}
\newpage
Changed
\begin{equation}\label{eq:xB}
	x_B=l_1\cdot\cos(\phi_n)+\sqrt{l_2^{2}-\left(l_1\cdot\sin(\phi_n)-e_1\right)^{2}}=\dfrac{-1+\sqrt{3}}{50}\approx 0.014641
\end{equation}

\begin{figure}[H]
	\centering
	\begin{tikzpicture}
		\begin{axis}[
			grid = major,
			axis equal image = false,
			width=16.5cm,
			]
			\addplot plot table {graphs/xB.dat};
		\end{axis}
	\end{tikzpicture}
	\caption{$ x_B $}
\end{figure}
%\newline
Changed
\begin{equation}\label{eq:yB}
	y_B=e_1=0.005
\end{equation}

\begin{figure}[H]
	\centering
	\begin{tikzpicture}
		\begin{axis}[
			grid = major,
			axis equal image = false,
			width=16.5cm,
			]
			\addplot plot table {graphs/yB.dat};
		\end{axis}
	\end{tikzpicture}
	\caption{$ y_B $}
\end{figure}

\newpage
Середина первого звена $ OA $:
TODO
\begin{equation}\label{eq:xl1}
	x_{OA}=\dfrac{x_O+x_A}{2}=\dfrac{0 + l_1\cdot\cos(\phi)}{2} = \dfrac{l_1\cdot\cos(\phi)}{2}
\end{equation}
TODO
\begin{figure}[H]
	\centering
	\begin{tikzpicture}
		\begin{axis}[
			grid = major,
			axis equal image = false,
			width=16.5cm,
			]
			\addplot plot table {graphs/8.dat};
		\end{axis}
	\end{tikzpicture}
\end{figure}
\newpage
\begin{equation}\label{eq:yl1}
	y_{OA}=\dfrac{y_O+y_A}{2}=\dfrac{0 + l_1\cdot\sin(\phi)}{2}=\dfrac{l_1\cdot\sin(\phi)}{2}
\end{equation}

\begin{figure}[H]
	\centering
	\begin{tikzpicture}
		\begin{axis}[
			grid = major,
			axis equal image = false,
			width=16.5cm,
			]
			\addplot plot table {graphs/9.dat};
		\end{axis}
	\end{tikzpicture}
\end{figure}
\newpage
Середина второго звена $ AB $:
OLD
\begin{multline}\label{eq:xl2}
	x_{AB}=\dfrac{l_1\cdot\cos(\phi) + 	l_1\cdot\cos(\phi)+l_2\cdot\cos\left(\arcsin\left(\dfrac{e_1-l_1\cdot\sin(\phi)}{l_2}\right)\right)}{2}=\\
	=\dfrac{2\cdot l_1\cdot\cos(\phi)+l_2\cdot\cos\left(\arcsin\left(\dfrac{e_1-l_1\cdot\sin(\phi)}{l_2}\right)\right)}{2}
\end{multline}

NEW
%\begin{equation}\label{eq:xl2}
%	x_{AB}=\dfrac{-l_1^{2}\sin(2\phi)+2l_{1}e_{1}\cos(\phi)}{4\sqrt{l_{2}^{2}-l_{1}^{2}\sin^{2}(\phi)+2l_{}}}
%\end{equation}


\begin{figure}[H]
	\centering
	\begin{tikzpicture}
		\begin{axis}[
			grid = major,
			axis equal image = false,
			width=16.5cm,
			]
			\addplot plot table {graphs/10.dat};
		\end{axis}
	\end{tikzpicture}
		\caption{$ x_{AB} $}
\end{figure}

%\newpage

\begin{equation}\label{eq:yl2}
	y_{AB}=\dfrac{y_A+y_{c_1}}{2}=\dfrac{l_1\cdot\sin(\phi) + 0}{2} = \dfrac{l_1\cdot\sin(\phi)}{2}
\end{equation}

\begin{figure}[H]
	\centering
	\begin{tikzpicture}
		\begin{axis}[
			grid = major,
			axis equal image = false,
			width=16.5cm,
			]
			\addplot plot table {graphs/11.dat};
		\end{axis}
	\end{tikzpicture}
	\caption{$ y_{AB} $}
\end{figure}
\newpage
Найдём производные $ A $, $OA$, $AB $ по $ \phi $:

\begin{equation}\label{eq:xAdphi}
	x_A'=-l1\cdot\sin(\phi)
\end{equation}

\begin{figure}[H]
	\centering
	\begin{tikzpicture}
		\begin{axis}[
			grid = major,
			axis equal image = false,
			width=16.5cm,
			]
			\addplot plot table {graphs/12.dat};
		\end{axis}
	\end{tikzpicture}
\end{figure}
\newpage
\begin{equation}\label{eq:yAdphi}
	y_A'=l1\cdot\cos(\phi)
\end{equation}

\begin{figure}[H]
	\centering
	\begin{tikzpicture}
		\begin{axis}[
			grid = major,
			axis equal image = false,
			width=16.5cm,
			]
			\addplot plot table {graphs/13.dat};
		\end{axis}
	\end{tikzpicture}
\end{figure}
\newpage
\begin{equation}\label{eq:xOAdphi}
	x_{OA}'=\dfrac{-l1\cdot\sin(\phi)}{2}
\end{equation}

\begin{figure}[H]
	\centering
	\begin{tikzpicture}
		\begin{axis}[
			grid = major,
			axis equal image = false,
			width=16.5cm,
			]
			\addplot plot table {graphs/14.dat};
		\end{axis}
	\end{tikzpicture}
\end{figure}
\newpage
\begin{equation}\label{eq:yOAdphi}
	y_{OA}'=\dfrac{l1\cdot\cos(\phi)}{2}
\end{equation}

\begin{figure}[H]
	\centering
	\begin{tikzpicture}
		\begin{axis}[
			grid = major,
			axis equal image = false,
			width=16.5cm,
			]
			\addplot plot table {graphs/15.dat};
		\end{axis}
	\end{tikzpicture}
\end{figure}
\newpage
OLD
\begin{equation}\label{eq:xABdphi}
	x_{AB}'=-l1\cdot\sin(\phi)+
	\dfrac{{l_2}^{2}\cdot \left(\dfrac{e_1}{2}-\dfrac{1}{2}\cdot l_2\cdot\sin(\phi) \right)\cdot\cos(\phi)}{4\cdot \sqrt{1-{\left(\dfrac{e_1}{2}-\dfrac{1}{2}\cdot l_2\cdot \sin(\phi) \right)}^{2}}}
\end{equation}

NEW

\begin{multline}
x_{AB}(\dfrac{1}{2} \sqrt{l_{2}^{2} - (l_1\sin(x) - e_1)^2} + l_1 \cos(x)) =\\ \frac{1}{2} (-(l_1^2 \cos^2(x))/\sqrt{l_2^2 - (l_1 \sin(x) - e_1)^2} - \dfrac{l_1^2 \cos^2(x) (l_1 \sin(x) - e_1)^2}{(l_2^2 - (l_1 \sin(x) - e_1)^2)^{\frac{3}{2}}} +\\ \dfrac{l_1 \sin(x) (l_1 \sin(x) - e_1)}{\sqrt{l_2^2 - (l_1 \sin(x) - e_1)^2}) - l_1 \cos(x)}
\end{multline}

\begin{figure}[H]
	\centering
	\begin{tikzpicture}
		\begin{axis}[
			grid = major,
			axis equal image = false,
			width=16.5cm,
			]
			\addplot plot table {graphs/16.dat};
		\end{axis}
	\end{tikzpicture}
\end{figure}
\newpage
\begin{equation}\label{eq:yABdphi}
	y_{AB}'=\dfrac{l_1\cdot\cos(\phi)}{2}
\end{equation}

\begin{figure}[H]
	\centering
	\begin{tikzpicture}
		\begin{axis}[
			grid = major,
			axis equal image = false,
			width=16.5cm,
			]
			\addplot plot table {graphs/17.dat};
		\end{axis}
	\end{tikzpicture}
\end{figure}
\newpage
Найдём вторые производные:

\begin{equation}\label{eq:xAdphi2}
	x_A''=-l_1\cdot\cos(\phi)
\end{equation}

\begin{figure}[H]
	\centering
	\begin{tikzpicture}
		\begin{axis}[
			grid = major,
			axis equal image = false,
			width=16.5cm,
			]
			\addplot plot table {graphs/18.dat};
		\end{axis}
	\end{tikzpicture}
\end{figure}
\newpage
\begin{equation}\label{eq:yAdphi2}
	y_A''=-l_1\cdot\sin(\phi)
\end{equation}

\begin{figure}[H]
	\centering
	\begin{tikzpicture}
		\begin{axis}[
			grid = major,
			axis equal image = false,
			width=16.5cm,
			]
			\addplot plot table {graphs/19.dat};
		\end{axis}
	\end{tikzpicture}
\end{figure}
\newpage
\begin{equation}\label{eq:xOAdphi2}
	x_{OA}''=\dfrac{-l_1\cdot\cos(\phi)}{2}
\end{equation}

\begin{figure}[H]
	\centering
	\begin{tikzpicture}
		\begin{axis}[
			grid = major,
			axis equal image = false,
			width=16.5cm,
			]
			\addplot plot table {graphs/20.dat};
		\end{axis}
	\end{tikzpicture}
\end{figure}
\newpage
\begin{equation}\label{eq:yOAdphi2}
	y_{OA}''=\dfrac{-l_1\cdot\sin(\phi)}{2}
\end{equation}

\begin{figure}[H]
	\centering
	\begin{tikzpicture}
		\begin{axis}[
			grid = major,
			axis equal image = false,
			width=16.5cm,
			]
			\addplot plot table {graphs/21.dat};
		\end{axis}
	\end{tikzpicture}
\end{figure}
\newpage
\begin{eqnarray}\label{eq:xABdphi2}
	x_{AB}''=\dfrac{1}{2}\cdot\Bigg(-\dfrac{{l_2}^{3}\cdot\cos^{2}(x)}{4\cdot\sqrt{1-\dfrac{1}{4}\cdot\left(e_1-l_2\cdot\sin(x)\right)^{2}}}-\\
	-\dfrac{{l_2}^{3}\cdot\cos^{2}(x)\cdot\left(e_1-l_2\cdot\sin(x)\right)^{2} }{16\cdot\left(1-\dfrac{1}{4}\cdot\left(e_1-l_2\cdot\sin(x)\right)^{2}\right)^{\frac{3}{2}}}-\\
	-\dfrac{{l_2}^{2}\cdot\sin(x)\cdot\left(e_1-l_2\cdot\sin(x)\right)}{4\cdot\sqrt{1-\dfrac{1}{4}\cdot\left(e_1-l_2\cdot\sin(x)\right)^{2}}}-2\cdot l_1\cdot\cos(x)\Bigg)
\end{eqnarray}

\begin{figure}[H]
	\centering
	\begin{tikzpicture}
		\begin{axis}[
			grid = major,
			axis equal image = false,
			width=16.5cm,
			]
			\addplot plot table {graphs/22.dat};
		\end{axis}
	\end{tikzpicture}
\end{figure}
\newpage	
%\begin{multline}\label{eq:xABdphi2}
%	x_{AB}''=\dfrac{1}{2}\cdot\left(
%	-\dfrac{l_2^{3}\cdot\cos^{2}(x)}{4\cdot\sqrt{1-\dfrac{1}{4}\cdot\left(e_1-l_2\cdot\sin(x)\right)^{2}}}-\\
%	-\dfrac{l_2^{3}\cdot\cos^{2}(x)\cdot\left(e_1-l_2\cdot\sin(x)\right)^{2} }{16\cdot\left(1-\dfrac{1}{4}\cdot\left(e_1-l_2\cdot\sin(x)\right)^{2}\right)^{\dfrac{3}{2}}}-\\
%	-\dfrac{l_2^{2}\cdot\sin(x)\cdot\left(e_1-l_2\cdot\sin(x)\right)}{4\cdot\sqrt{1-\dfrac{1}{4}\cdot\left(e_1-l_2\cdot\sin(x)\right)^{2}}}-2\cdot l_1\cdot\cos(x)\right)
%\end{multline}

\begin{equation}\label{eq:yABdphi2}
	y_{AB}''=\dfrac{-l_1\cdot\sin(\phi)}{2}
\end{equation}

\begin{figure}[H]
	\centering
	\begin{tikzpicture}
		\begin{axis}[	
			grid = major,
			axis equal image = false,
			width=16.5cm,
			]
			\addplot plot table {graphs/25.dat};
		\end{axis}
	\end{tikzpicture}
\end{figure}